EvmCompiler/Assembly/Semantics.lean
@@ -9,13 +9,6 @@ namespace Assembly
 abbrev EVMState := EvmYul.EVM.State
 abbrev EVMException := EvmYul.EVM.ExecutionException
 
-inductive HaltKind where
-  | stop
-  | return
-  | revert
-  | selfdestruct
-  deriving DecidableEq, Repr
-
 structure Halt where
   kind : HaltKind
   state : EVMState
@@ -27,35 +20,12 @@ inductive StepResult where
 
 namespace HaltKind
 
-def argCount : HaltKind → Nat
-  | .stop => 0
-  | .return => 2
-  | .revert => 2
-  | .selfdestruct => 1
-
-def toPrimOp : HaltKind → PrimOp
-  | .stop => .stop
-  | .return => .return
-  | .revert => .revert
-  | .selfdestruct => .selfdestruct
-
 def output (kind : HaltKind) (state : EVMState) : ByteArray :=
   match kind with
   | .stop | .selfdestruct => .empty
   | .return | .revert => state.toMachineState.H_return
 
 end HaltKind
-
-namespace PrimOp
-
-def haltKind? : PrimOp → Option HaltKind
-  | .stop => some .stop
-  | .return => some .return
-  | .revert => some .revert
-  | .selfdestruct => some .selfdestruct
-  | _ => none
-
-end PrimOp
 
 namespace TargetInstr
 
